Give external events a semantics.
External events are passed a list of values of base type, and are
allowed to pass back a value of base type. In the semantics we model
this with non-determinism, since we do not want to make any assumptions
about the nature of the external event.

IL/IL.v
@@ -1,9 +1,16 @@
 Require Import List.
-Require Export Util Relations Get Drop Var Val Exp Env Map CSet AutoIndTac MoreList OptionMap.
+Require Export Util Relations Get Drop Var Val Exp Env Map CSet AutoIndTac MoreList OptionMap Events.
 
 Set Implicit Arguments.
 
 Open Scope map_scope.
+
+Ltac stuck2 :=
+  let σ := fresh "σ" in
+  let A := fresh "A" in
+  let v := fresh "v" in
+  let evt := fresh "evt" in
+  intros [v [evt A]]; inv A; isabsurd.
 
 (** * Intermediate Language IL *)
 
@@ -14,33 +21,35 @@ Notation "'args'" := (list exp) (at level 0).
 (** ... while [params] is the type of the list of formal parameters *)
 Notation "'params'" := (list var) (at level 0).
 
+
 Inductive stmt : Type :=
 | stmtExp    (x : var) (e: exp) (s : stmt) : stmt
 | stmtIf     (e : exp) (s : stmt) (t : stmt) : stmt
 | stmtGoto   (l : lab) (Y:args) : stmt
-| stmtReturn (e : exp) : stmt 
-(* block f Z : rt = s in b *)    
+| stmtReturn (e : exp) : stmt
+| stmtExtern (x : var) (f:external) (Y:args) (s:stmt)
+(* block f Z : rt = s in b *)
 | stmtLet    (Z:params) (s : stmt) (t : stmt) : stmt.
 
 Inductive notOccur (G:set var) : stmt -> Prop :=
-  | ncExp x e s 
-    : x ∉ G 
-      -> notOccur G s 
-      -> Exp.notOccur G e 
+  | ncExp x e s
+    : x ∉ G
+      -> notOccur G s
+      -> Exp.notOccur G e
       -> notOccur G (stmtExp x e s)
-  | ncIf e s t 
-    : Exp.notOccur G e 
-      -> notOccur G s 
-      -> notOccur G t 
+  | ncIf e s t
+    : Exp.notOccur G e
+      -> notOccur G s
+      -> notOccur G t
       -> notOccur G (stmtIf e s t)
   | ncRet e : Exp.notOccur G e -> notOccur G (stmtReturn e)
-  | ncGoto l (Y:list exp) 
-    : (forall n e, get Y n e -> Exp.notOccur G e) 
+  | ncGoto l (Y:list exp)
+    : (forall n e, get Y n e -> Exp.notOccur G e)
       -> notOccur G (stmtGoto l Y)
-  | ncLet s Z t 
-    : of_list Z ∩ G [=] ∅ 
-      -> notOccur G s 
-      -> notOccur G t 
+  | ncLet s Z t
+    : of_list Z ∩ G [=] ∅
+      -> notOccur G s
+      -> notOccur G t
       -> notOccur G (stmtLet Z s t).
 
 Fixpoint freeVars (s:stmt) : set var :=
@@ -49,6 +58,7 @@ Fixpoint freeVars (s:stmt) : set var :=
     | stmtIf e s1 s2 => freeVars s1 ∪ freeVars s2 ∪ Exp.freeVars e
     | stmtGoto l Y => list_union (List.map Exp.freeVars Y)
     | stmtReturn e => Exp.freeVars e
+    | stmtExtern x f Y s => (freeVars s \ {{x}}) ∪ list_union (List.map Exp.freeVars Y)
     | stmtLet Z s1 s2 => (freeVars s1 \ of_list Z) ∪ freeVars s2
   end.
 
@@ -58,6 +68,7 @@ Fixpoint occurVars (s:stmt) : set var :=
     | stmtIf e s1 s2 => occurVars s1 ∪ occurVars s2 ∪ Exp.freeVars e
     | stmtGoto l Y => list_union (List.map Exp.freeVars Y)
     | stmtReturn e => Exp.freeVars e
+    | stmtExtern x f Y s => freeVars s ∪ {{x}} ∪ list_union (List.map Exp.freeVars Y)
     | stmtLet Z s1 s2 => freeVars s1 ∪ freeVars s2 ∪ of_list Z
   end.
 
@@ -67,22 +78,24 @@ Fixpoint rename (ϱ:env var) (s:stmt) : stmt :=
     | stmtIf e s t => stmtIf (rename_exp ϱ e) (rename ϱ s) (rename ϱ t)
     | stmtGoto l Y => stmtGoto l (List.map (rename_exp ϱ) Y)
     | stmtReturn e => stmtReturn (rename_exp ϱ e)
+    | stmtExtern x f e s => stmtExtern (ϱ x) f (List.map (rename_exp ϱ) e) (rename ϱ s)
     | stmtLet Z s t => stmtLet (lookup_list ϱ Z) (rename ϱ s) (rename ϱ t)
-  end.  
+  end.
 
 Fixpoint label_closed (n:nat) (s:stmt) : Prop :=
   match s with
-    | stmtExp _ e s => label_closed n s
+    | stmtExp _ _ s => label_closed n s
     | stmtIf _ s t => label_closed n s /\ label_closed n t
     | stmtGoto l _ => counted l < n
     | stmtReturn _ => True
+    | stmtExtern _ _ _ s => label_closed n s
     | stmtLet _ s t => label_closed (S n) s /\ label_closed (S n) t
   end.
 
 Lemma notOccur_incl G G' s
   : G' ⊆ G -> notOccur G s -> notOccur G' s.
 Proof.
-  intros A B. general induction B; 
+  intros A B. general induction B;
               eauto using notOccur, incl_not_member, incl_meet_empty,
               Exp.notOccur_antitone.
 Qed.
@@ -99,10 +112,10 @@ Qed.
 Add Parametric Morphism : notOccur with
   signature Equal ==> eq ==> iff as eq_cset_notOccur_morphism.
 Proof.
-  intros. split; intros. 
-  assert (Subset y x); intuition. 
+  intros. split; intros.
+  assert (Subset y x); intuition.
   rewrite H1; eauto.
-  assert (Subset x y); intuition. 
+  assert (Subset x y); intuition.
   rewrite H1; eauto.
 Qed.
 
@@ -121,58 +134,68 @@ Module F.
   Definition labenv := list block.
   Definition state : Type := (labenv * onv val * stmt)%type.
 
-  Inductive step : state -> state -> Prop :=
+  Inductive step : state -> event -> state -> Prop :=
   | stepExp L E x e b v
     (def:exp_eval E e = Some v)
-    : step (L, E, stmtExp x e b) (L, E[x<-Some v], b)
+    : step (L, E, stmtExp x e b) EvtTau (L, E[x<-Some v], b)
 
-  | stepIfT L E 
+  | stepIfT L E
     e (b1 b2 : stmt) v
     (def:exp_eval E e = Some v)
     (condTrue: val2bool v = true)
-    : step (L, E, stmtIf e b1 b2) (L, E, b1)
-    
+    : step (L, E, stmtIf e b1 b2) EvtTau (L, E, b1)
+
   | stepIfF L E
     e (b1 b2:stmt) v
     (def:exp_eval E e = Some v)
     (condFalse: val2bool v = false)
-    : step (L, E, stmtIf e b1 b2) (L, E, b2)
-    
+    : step (L, E, stmtIf e b1 b2) EvtTau (L, E, b2)
+
   | stepGoto L E l Y blk vl
     (Ldef:get L (counted l) blk)
     (len:length (block_Z blk) = length Y)
     (def:omap (exp_eval E) Y = Some vl) E'
     (updOk:(block_E blk) [block_Z blk <-- List.map Some vl] = E')
     : step  (L, E, stmtGoto l Y)
+            EvtTau
             (drop (counted l) L, E', block_s blk)
 
-  | stepLet L E 
-    s Z (t:stmt) 
-    : step (L, E, stmtLet Z s t) (blockI E Z s::L, E, t).
-  
-  Lemma step_functional :
-    functional step.
+  | stepLet L E
+    s Z (t:stmt)
+    : step (L, E, stmtLet Z s t) EvtTau (blockI E Z s::L, E, t)
+
+  | stepExtern L E x f Y s vl v
+    (def:omap (exp_eval E) Y = Some vl)
+    : step  (L, E, stmtExtern x f Y s)
+            (EvtExtern (ExternI f vl v))
+            (L, E[x <- Some v], s).
+
+  Lemma step_internally_deterministic :
+    internally_deterministic step.
   Proof.
-    induction 1; inversion 1; intros; subst; repeat get_functional; try congruence.
+    hnf; intros.
+    inv H; inv H0; split; eauto; try get_functional; try congruence.
   Qed.
 
-  Lemma step_dec 
+  Lemma step_dec
   : reddec step.
   Proof.
     hnf; intros. destruct x as [[L V] []].
-    - case_eq (exp_eval V e); intros. left. eauto using step.
+    - case_eq (exp_eval V e); intros. left. do 2 eexists. eauto 20 using step.
       right. stuck.
-    - case_eq (exp_eval V e); intros. 
-      left. case_eq (val2bool v); intros; eauto using step.
+    - case_eq (exp_eval V e); intros.
+      left. case_eq (val2bool v); intros; do 2 eexists; eauto using step.
       right. stuck.
     - destruct (get_dec L (counted l)) as [[blk A]|?].
       decide (length (block_Z blk) = length Y).
       case_eq (omap (exp_eval V) Y); intros; try now (right; stuck).
-      + left. econstructor. econstructor; eauto.
-      + right. stuck. get_functional; subst; eauto.
-      + right. stuck. eauto.
-    - right. stuck.
-    - left. eauto using step.
+      + left. do 2 eexists. econstructor; eauto.
+      + right. stuck2. get_functional; subst; eauto.
+      + right. stuck2. eauto.
+    - right. stuck2.
+    - case_eq (omap (exp_eval V) Y); intros; try now (right; stuck).
+      left; eexists (EvtExtern (ExternI f l 0)). eexists; eauto using step.
+    - left. eexists. eauto using step.
   Qed.
 
 End F.
@@ -189,92 +212,73 @@ Module I.
   Definition labenv := list block.
   Definition state : Type := (labenv * onv val * stmt)%type.
 
-  Inductive step : state -> state -> Prop :=
+  Inductive step : state -> event -> state -> Prop :=
   | stepExp L E x e b v
     (def:exp_eval E e = Some v)
-    : step (L, E, stmtExp x e b) (L, E[x<-Some v], b)
+    : step (L, E, stmtExp x e b) EvtTau (L, E[x<-Some v], b)
 
-  | stepIfT L E 
+  | stepIfT L E
     e (b1 b2 : stmt) v
     (def:exp_eval E e = Some v)
     (condTrue: val2bool v = true)
-    : step (L, E, stmtIf e b1 b2) (L, E, b1)
-    
+    : step (L, E, stmtIf e b1 b2) EvtTau (L, E, b1)
+
   | stepIfF L E
     e (b1 b2:stmt) v
     (def:exp_eval E e = Some v)
     (condFalse: val2bool v = false)
-    : step (L, E, stmtIf e b1 b2) (L, E, b2)
-    
+    : step (L, E, stmtIf e b1 b2) EvtTau (L, E, b2)
+
   | stepGoto L E l Y blk vl
     (Ldef:get L (counted l) blk)
     (len:length (block_Z blk) = length Y)
     (def:omap (exp_eval E) Y = Some vl) E'
     (updOk:E[block_Z blk  <-- List.map Some vl] = E')
     : step  (L, E, stmtGoto l Y)
+            EvtTau
             (drop (counted l) L, E', block_s blk)
+
 
   | stepLet L E
     s Z (b:stmt)
-    : step (L, E, stmtLet Z s b) (blockI Z s::L, E, b).
-  
-  Lemma step_functional : functional step.
+    : step (L, E, stmtLet Z s b) EvtTau (blockI Z s::L, E, b)
+
+  | stepExtern L E x f Y s vl v
+    (def:omap (exp_eval E) Y = Some vl)
+    : step  (L, E, stmtExtern x f Y s)
+            (EvtExtern (ExternI f vl v))
+            (L, E[x <- Some v], s).
+
+
+  Lemma step_internally_deterministic :
+    internally_deterministic step.
   Proof.
-    hnf.
-    induction 1; inversion 1; intros; subst; repeat get_functional; try congruence.
+    hnf; intros.
+    inv H; inv H0; split; eauto; try get_functional; try congruence.
   Qed.
 
-  Lemma step_dec 
+  Lemma step_dec
   : reddec step.
   Proof.
     hnf; intros. destruct x as [[L V] []].
-    - case_eq (exp_eval V e); intros. left. eauto using step.
+    - case_eq (exp_eval V e); intros. left. do 2 eexists. eauto 20 using step.
       right. stuck.
-    - case_eq (exp_eval V e); intros. 
-      left. case_eq (val2bool v); intros; eauto using step.
+    - case_eq (exp_eval V e); intros.
+      left. case_eq (val2bool v); intros; do 2 eexists; eauto using step.
       right. stuck.
     - destruct (get_dec L (counted l)) as [[blk A]|?].
       decide (length (block_Z blk) = length Y).
       case_eq (omap (exp_eval V) Y); intros; try now (right; stuck).
-      + left. econstructor. econstructor; eauto.
-      + right. stuck. get_functional; subst; eauto.
-      + right. stuck. eauto.
-    - right. stuck.
-    - left. eauto using step.
+      + left. do 2 eexists. econstructor; eauto.
+      + right. stuck2. get_functional; subst; eauto.
+      + right. stuck2. eauto.
+    - right. stuck2.
+    - case_eq (omap (exp_eval V) Y); intros; try now (right; stuck).
+      left; eexists (EvtExtern (ExternI f l 0)). eexists; eauto using step.
+    - left. eexists. eauto using step.
   Qed.
 
 End I.
-
-Class StateType S := {
-  step : S -> S -> Prop;
-  result : S -> option val;
-  step_dec : reddec step;
-  step_functional : functional step
-}.
-
-Definition state_result X (s:X*onv val*stmt) : option val :=
-  match s with
-    | (_, stmtExp _ _ _) => None
-    | (_, stmtIf _ _ _) => None
-    | (_, stmtGoto _ _) => None
-    | (_, E, stmtReturn e) => exp_eval E e
-    | (_, stmtLet _ _ _) => None
-  end.
-
-Instance statetype_F : StateType F.state := {
-  step := F.step;
-  result := (@state_result F.labenv);
-  step_dec := F.step_dec;
-  step_functional := F.step_functional
-}.
-
-
-Instance statetype_I : StateType I.state := {
-  step := I.step;
-  result := (@state_result I.labenv);
-  step_dec := I.step_dec;
-  step_functional := I.step_functional
-}. 
 
 Fixpoint labenvRmE (L:F.labenv) : I.labenv
   :=
@@ -283,9 +287,8 @@ Fixpoint labenvRmE (L:F.labenv) : I.labenv
     | F.blockI E Z s::L => I.blockI Z s :: labenvRmE L
   end.
 
-(* 
+(*
 *** Local Variables: ***
 *** coq-load-path: (("../" "Lvc")) ***
 *** End: ***
 *)
-
