IL/StateType.v
@@ -1,0 +1,40 @@
+Require Import List.
+Require Export Util Relations Get Drop Var Val Exp Env Map CSet AutoIndTac MoreList OptionMap Events IL.
+
+Set Implicit Arguments.
+
+
+Class StateType S := {
+  step : S -> event -> S -> Prop;
+  result : S -> option val;
+  step_dec : reddec step;
+  step_internally_deterministic : internally_deterministic step
+}.
+
+Definition state_result X (s:X*onv val*stmt) : option val :=
+  match s with
+    | (_, E, stmtReturn e) => exp_eval E e
+    | _ => None
+  end.
+
+Instance statetype_F : StateType F.state := {
+  step := F.step;
+  result := (@state_result F.labenv);
+  step_dec := F.step_dec;
+  step_internally_deterministic := F.step_internally_deterministic
+}.
+
+
+Instance statetype_I : StateType I.state := {
+  step := I.step;
+  result := (@state_result I.labenv);
+  step_dec := I.step_dec;
+  step_internally_deterministic := I.step_internally_deterministic
+}.
+
+
+(*
+*** Local Variables: ***
+*** coq-load-path: (("../" "Lvc")) ***
+*** End: ***
+*)
